contrib/field/Field_Theory.v
@@ -65,10 +65,10 @@ Definition eqExprA := Eval Compute in eqExprA_O.
 
 (**** Generation of the multiplier ****)
 
-Fixpoint mult_of_list [e:(list ExprA)]: ExprA :=
+Fixpoint mult_of_list [e:(listT ExprA)]: ExprA :=
   Cases e of
   | nil => EAone
-  | (cons e1 l1) => (EAmult e1 (mult_of_list l1))
+  | (consT e1 l1) => (EAmult e1 (mult_of_list l1))
   end.
 
 Section Theory_of_fields.
@@ -189,7 +189,7 @@ Save.
 
 (**** ExprA --> A ****)
 
-Fixpoint interp_ExprA [lvar:(list (Sprod AT nat));e:ExprA] : AT :=
+Fixpoint interp_ExprA [lvar:(listT (Sprod AT nat));e:ExprA] : AT :=
   Cases e of
   | EAzero         => AzeroT
   | EAone          => AoneT
@@ -254,7 +254,7 @@ Fixpoint assoc [e:ExprA] : ExprA :=
   end.
 
 Lemma merge_mult_correct1:
-  (e1,e2,e3:ExprA)(lvar:(list (Sprod AT nat)))
+  (e1,e2,e3:ExprA)(lvar:(listT (Sprod AT nat)))
   (interp_ExprA lvar (merge_mult (EAmult e1 e2) e3))==
   (interp_ExprA lvar (EAmult e1 (merge_mult e2 e3))).
 Proof.
@@ -268,7 +268,7 @@ Unfold 1 merge_mult;Fold merge_mult;
 Save.
 
 Lemma merge_mult_correct:
-  (e1,e2:ExprA)(lvar:(list (Sprod AT nat)))
+  (e1,e2:ExprA)(lvar:(listT (Sprod AT nat)))
     (interp_ExprA lvar (merge_mult e1 e2))==
     (interp_ExprA lvar (EAmult e1 e2)).
 Proof.
@@ -284,7 +284,7 @@ Intro H3;Rewrite H3;Rewrite <-H2;
 Ring.
 Save.
 
-Lemma assoc_mult_correct1:(e1,e2:ExprA)(lvar:(list (Sprod AT nat)))
+Lemma assoc_mult_correct1:(e1,e2:ExprA)(lvar:(listT (Sprod AT nat)))
   (AmultT (interp_ExprA lvar (assoc_mult e1)) 
          (interp_ExprA lvar (assoc_mult e2)))==
   (interp_ExprA lvar (assoc_mult (EAmult e1 e2))).
@@ -295,7 +295,7 @@ Rewrite <-(H e0 lvar);Simpl;Rewrite merge_mult_correct;Simpl;
 Save.
 
 Lemma assoc_mult_correct:
-  (e:ExprA)(lvar:(list (Sprod AT nat)))
+  (e:ExprA)(lvar:(listT (Sprod AT nat)))
     (interp_ExprA lvar (assoc_mult e))==(interp_ExprA lvar e).
 Proof.
 Induction e;Auto;Intros.
@@ -317,7 +317,7 @@ Simpl;Rewrite (H0 lvar);Auto.
 Save.
 
 Lemma merge_plus_correct1:
-  (e1,e2,e3:ExprA)(lvar:(list (Sprod AT nat)))
+  (e1,e2,e3:ExprA)(lvar:(listT (Sprod AT nat)))
   (interp_ExprA lvar (merge_plus (EAplus e1 e2) e3))==
   (interp_ExprA lvar (EAplus e1 (merge_plus e2 e3))).
 Proof.
@@ -331,7 +331,7 @@ Unfold 1 merge_plus;Fold merge_plus;
 Save.
 
 Lemma merge_plus_correct:
-  (e1,e2:ExprA)(lvar:(list (Sprod AT nat)))
+  (e1,e2:ExprA)(lvar:(listT (Sprod AT nat)))
     (interp_ExprA lvar (merge_plus e1 e2))==
     (interp_ExprA lvar (EAplus e1 e2)).
 Proof.
@@ -346,7 +346,7 @@ Intro H3;Rewrite H3;Rewrite <-H2;Rewrite merge_plus_correct1;Simpl;Ring.
 Ring.
 Save.
 
-Lemma assoc_plus_correct:(e1,e2:ExprA)(lvar:(list (Sprod AT nat)))
+Lemma assoc_plus_correct:(e1,e2:ExprA)(lvar:(listT (Sprod AT nat)))
   (AplusT (interp_ExprA lvar (assoc e1)) (interp_ExprA lvar (assoc e2)))==
   (interp_ExprA lvar (assoc (EAplus e1 e2))).
 Proof.
@@ -356,7 +356,7 @@ Rewrite <-(H e0 lvar);Simpl;Rewrite merge_plus_correct;Simpl;
 Save.
 
 Lemma assoc_correct:
-  (e:ExprA)(lvar:(list (Sprod AT nat)))
+  (e:ExprA)(lvar:(listT (Sprod AT nat)))
     (interp_ExprA lvar (assoc e))==(interp_ExprA lvar e).
 Proof.
 Induction e;Auto;Intros.
@@ -429,7 +429,7 @@ Fixpoint distrib_main [e:ExprA] : ExprA :=
 Definition distrib [e:ExprA] : ExprA := (distrib_main (distrib_EAopp e)).
 
 Lemma distrib_mult_right_correct:
-  (e1,e2:ExprA)(lvar:(list (Sprod AT nat)))
+  (e1,e2:ExprA)(lvar:(listT (Sprod AT nat)))
      (interp_ExprA lvar (distrib_mult_right e1 e2))==
      (AmultT (interp_ExprA lvar e1) (interp_ExprA lvar e2)).
 Proof.
@@ -439,7 +439,7 @@ Rewrite AmultT_sym;Rewrite AmultT_AplusT_distr;
 Save.
 
 Lemma distrib_mult_left_correct:
-  (e1,e2:ExprA)(lvar:(list (Sprod AT nat)))
+  (e1,e2:ExprA)(lvar:(listT (Sprod AT nat)))
      (interp_ExprA lvar (distrib_mult_left e1 e2))==
      (AmultT (interp_ExprA lvar e1)  (interp_ExprA lvar e2)).
 Proof.
@@ -460,7 +460,7 @@ Rewrite distrib_mult_right_correct;Simpl;Apply AmultT_sym.
 Save.
 
 Lemma distrib_correct:
-  (e:ExprA)(lvar:(list (Sprod AT nat)))
+  (e:ExprA)(lvar:(listT (Sprod AT nat)))
     (interp_ExprA lvar (distrib e))==(interp_ExprA lvar e).
 Proof.
 Induction e;Intros;Auto.
@@ -475,7 +475,7 @@ Save.
 (**** Multiplication by the inverse product ****)
 
 Lemma mult_eq:
-  (e1,e2,a:ExprA)(lvar:(list (Sprod AT nat)))
+  (e1,e2,a:ExprA)(lvar:(listT (Sprod AT nat)))
     ~((interp_ExprA lvar a)==AzeroT)->
       (interp_ExprA lvar (EAmult a e1))==(interp_ExprA lvar (EAmult a e2))->
         (interp_ExprA lvar e1)==(interp_ExprA lvar e2).
@@ -499,7 +499,7 @@ Definition multiply [e:ExprA] : ExprA :=
   end.
 
 Lemma multiply_aux_correct:
-  (a,e:ExprA)(lvar:(list (Sprod AT nat)))
+  (a,e:ExprA)(lvar:(listT (Sprod AT nat)))
     (interp_ExprA lvar (multiply_aux a e))==
     (AmultT (interp_ExprA lvar a) (interp_ExprA lvar e)).
 Proof.
@@ -508,7 +508,7 @@ Induction e;Simpl;Intros;Try (Rewrite merge_mult_correct);Auto.
 Save.
 
 Lemma multiply_correct:
-  (e:ExprA)(lvar:(list (Sprod AT nat)))
+  (e:ExprA)(lvar:(listT (Sprod AT nat)))
     (interp_ExprA lvar (multiply e))==(interp_ExprA lvar e).
 Proof.
   Induction e;Simpl;Auto.
@@ -556,7 +556,7 @@ Fixpoint inverse_simplif [a,e:ExprA] : ExprA :=
   end.
 
 Lemma monom_remove_correct:(e,a:ExprA)
-  (lvar:(list (Sprod AT nat)))~((interp_ExprA lvar a)==AzeroT)->
+  (lvar:(listT (Sprod AT nat)))~((interp_ExprA lvar a)==AzeroT)->
   (interp_ExprA lvar (monom_remove a e))==
   (AmultT (interp_ExprA lvar a) (interp_ExprA lvar e)).
 Proof.
@@ -583,7 +583,7 @@ Unfold monom_remove;Case (eqExprA (EAvar n) (EAinv a));Intros;
 Save.
 
 Lemma monom_simplif_rem_correct:(a,e:ExprA)
-  (lvar:(list (Sprod AT nat)))~((interp_ExprA lvar a)==AzeroT)->
+  (lvar:(listT (Sprod AT nat)))~((interp_ExprA lvar a)==AzeroT)->
   (interp_ExprA lvar (monom_simplif_rem a e))==
   (AmultT (interp_ExprA lvar a) (interp_ExprA lvar e)).
 Proof.
@@ -595,7 +595,7 @@ Ring.
 Save.
 
 Lemma monom_simplif_correct:(e,a:ExprA)
-  (lvar:(list (Sprod AT nat)))~((interp_ExprA lvar a)==AzeroT)->
+  (lvar:(listT (Sprod AT nat)))~((interp_ExprA lvar a)==AzeroT)->
   (interp_ExprA lvar (monom_simplif a e))==(interp_ExprA lvar e).
 Proof.
 Induction e;Intros;Auto.
@@ -605,7 +605,7 @@ Simpl;Trivial.
 Save.
 
 Lemma inverse_correct:
-  (e,a:ExprA)(lvar:(list (Sprod AT nat)))~((interp_ExprA lvar a)==AzeroT)->
+  (e,a:ExprA)(lvar:(listT (Sprod AT nat)))~((interp_ExprA lvar a)==AzeroT)->
     (interp_ExprA lvar (inverse_simplif a e))==(interp_ExprA lvar e).
 Proof.
 Induction e;Intros;Auto.
