contrib/field/Field_Tactic.v
@@ -17,7 +17,7 @@ Require Export Field_Theory.
 Recursive Tactic Definition MemAssoc var lvar :=
   Match lvar With
   | [(nil ?)] -> false
-  | [(cons ? ?1 ?2)] ->
+  | [(consT ? ?1 ?2)] ->
     (Match ?1==var With
      | [?1== ?1] -> true
      | _ -> (MemAssoc var ?2)).
@@ -45,7 +45,7 @@ Recursive Tactic Definition SeekVarAux FT lvar trm :=
     Let res = (MemAssoc ?1 lvar) In
     Match res With
     | [(true)] -> lvar
-    | [(false)] -> '(cons AT ?1 lvar).
+    | [(false)] -> '(consT AT ?1 lvar).
 
 Tactic Definition SeekVar FT trm :=
   Let AT = Eval Compute in (A FT) In
@@ -54,9 +54,9 @@ Tactic Definition SeekVar FT trm :=
 Recursive Tactic Definition NumberAux lvar cpt :=
   Match lvar With
   | [(nil ?1)] -> '(nil (Sprod ?1 nat))
-  | [(cons ?1 ?2 ?3)] ->
+  | [(consT ?1 ?2 ?3)] ->
     Let l2 = (NumberAux ?3 '(S cpt)) In
-    '(cons (Sprod ?1 nat) (Spair ?1 nat ?2 cpt) l2).
+    '(consT (Sprod ?1 nat) (Spair ?1 nat ?2 cpt) l2).
 
 Tactic Definition Number lvar := (NumberAux lvar O).
 
@@ -67,7 +67,7 @@ Tactic Definition BuildVarList FT trm :=
 Recursive Tactic Definition Assoc elt lst :=
   Match lst With
   | [(nil ?)] -> Fail
-  | [(cons (Sprod ? nat) (Spair ? nat ?1 ?2) ?3)] ->
+  | [(consT (Sprod ? nat) (Spair ? nat ?1 ?2) ?3)] ->
     Match elt== ?1 With
     | [?1== ?1] -> ?2
     | _ -> (Assoc elt ?3).
@@ -110,22 +110,22 @@ Recursive Tactic Definition interp_A FT lvar trm :=
 Recursive Tactic Definition Remove e l :=
   Match l With
   | [(nil ?)] -> l
-  | [(cons ?1 e ?2)] -> ?2
-  | [(cons ?1 ?2 ?3)] ->
+  | [(consT ?1 e ?2)] -> ?2
+  | [(consT ?1 ?2 ?3)] ->
     Let nl = (Remove e ?3) In
-    '(cons ?1 ?2 nl).
+    '(consT ?1 ?2 nl).
 
 Recursive Tactic Definition Union l1 l2 :=
   Match l1 With
   | [(nil ?)] -> l2
-  | [(cons ?1 ?2 ?3)] ->
+  | [(consT ?1 ?2 ?3)] ->
     Let nl2 = (Remove ?2 l2) In
     Let nl = (Union ?3 nl2) In
-    '(cons ?1 ?2 nl).
+    '(consT ?1 ?2 nl).
 
 Recursive Tactic Definition RawGiveMult trm :=
   Match trm With
-  | [(EAinv ?1)] -> '(cons ExprA ?1 (nil ExprA))
+  | [(EAinv ?1)] -> '(consT ExprA ?1 (nil ExprA))
   | [(EAopp ?1)] -> (RawGiveMult ?1)
   | [(EAplus ?1 ?2)] ->
     Let l1 = (RawGiveMult ?1)
@@ -134,7 +134,7 @@ Recursive Tactic Definition RawGiveMult trm :=
   | [(EAmult ?1 ?2)] ->
     Let l1 = (RawGiveMult ?1)
     And l2 = (RawGiveMult ?2) In
-    Eval Compute in (app ExprA l1 l2)
+    Eval Compute in (appT ExprA l1 l2)
   | _ -> '(nil ExprA).
 
 Tactic Definition GiveMult trm :=
